change nodes to footprint

node.dfy
@@ -3,40 +3,40 @@ include "utils.dfy"
 class Node {
   var prev: Node
   var next:  Node
-  ghost var nodes: seq<Node>
+  ghost var footprint: seq<Node>
   // int nat seq<Node> map<node> set<Node>
   constructor()
     ensures Valid(this)
-    ensures this == this.nodes[0]
+    ensures this == this.footprint[0]
     ensures Singleton(this)
   {
     prev := this;
     next := this;
-    nodes := [ this ];
+    footprint := [ this ];
   }
 }
 
 // implies that this node is not connected to any other nodes.
 predicate Singleton(n: Node)
   requires Valid(n)
-  ensures Singleton(n) ==> n.nodes == [ n ]
-  reads n, n.nodes
+  ensures Singleton(n) ==> n.footprint == [ n ]
+  reads n, n.footprint
 {
-  ghost var i := IndexOf(n.nodes, n);
-  assert n.next == n.nodes[(i + 1) % |n.nodes|];
+  ghost var i := IndexOf(n.footprint, n);
+  assert n.next == n.footprint[(i + 1) % |n.footprint|];
   n.prev == n.next == n
 }
 
 // Validity of a link in a cicular linked list
 ghost predicate Valid(node: Node)
   reads node
-  reads node.nodes
+  reads node.footprint
 {
-  var nodes := node.nodes;
+  var nodes := node.footprint;
 
   && |nodes| > 0
   && (node in multiset(nodes)) // self is present in the set of nodes
-  && (forall node' {:trigger node'.nodes == nodes} :: node' in nodes ==>  node'.nodes == nodes) // all nodes are same in the chain
+  && (forall node' {:trigger node'.footprint == nodes} :: node' in nodes ==>  node'.footprint == nodes) // all nodes are same in the chain
   && NoDupes(nodes) // no duplicates in the chain (they are pointers)
   && (forall i :: 0 <= i < |nodes| - 1 ==> nodes[i].next == nodes[i+1]) // assert that every next pointer is in the next index
   && nodes[|nodes|-1].next == nodes[0] // except the very last one that wraps to the first one
